proof/invariant-abstract/X64/ArchAcc_AI.thy
@@ -795,19 +795,23 @@ definition
       \<lambda>s. (\<exists>\<rhd> (p && ~~ mask pdpt_bits) and pdpte_at p) s \<and>
           wellformed_pdpte pdpte \<and> valid_pdpte pdpte s"
 
-lemma ucast_mask_asid_low_bits [simp]:
-  "ucast ((asid::word64) && mask asid_low_bits) = (ucast asid :: 9 word)"
-  apply (rule word_eqI)
-  apply (clarsimp simp: word_size nth_ucast asid_low_bits_def)
-  done
-
-
 lemma ucast_ucast_asid_high_bits [simp]:
   "ucast (ucast (asid_high_bits_of asid)::word64) = asid_high_bits_of asid"
   apply (rule word_eqI)
   apply (clarsimp simp: word_size nth_ucast asid_low_bits_def)
   done
 
+lemma ucast_ucast_asid_low_bits [simp]:
+  "ucast (ucast (asid_low_bits_of asid)::word64) = asid_low_bits_of asid"
+  apply (rule word_eqI)
+  apply (clarsimp simp: word_size nth_ucast asid_low_bits_def)
+  done
+
+lemma ucast_mask_asid_low_bits [simp]:
+  "ucast ((asid::word64) && mask asid_low_bits) = (ucast asid :: 9 word)"
+  apply (rule word_eqI)
+  apply (clarsimp simp: word_size nth_ucast asid_low_bits_def)
+  done
 
 lemma mask_asid_low_bits_ucast_ucast:
   "((asid::word64) && mask asid_low_bits) = ucast (ucast asid :: 9 word)"
