proof/invariant-abstract/X64/ArchBits_AI.thy
@@ -39,7 +39,7 @@ lemmas is_cap_simps = is_cap_simps is_arch_cap_simps
 lemmas valid_cap_def = valid_cap_def[simplified valid_arch_cap_def]
 
 lemmas valid_cap_simps =
-  valid_cap_def[split_simps cap.split arch_cap.split]
+  valid_cap_def[split_simps cap.split arch_cap.split, simplified wellformed_mapdata_def]
 
 end
 
